up to decreases

src/Distributions/DiscreteLaplace/Model.dfy
@@ -16,24 +16,23 @@ module DiscreteLaplace.Model {
    Definitions
   ************/
 
-  ghost function Sample(scale: Rationals.Rational): Monad.Hurd<int>
+  ghost opaque function Sample(scale: Rationals.Rational): Monad.Hurd<int>
     requires scale.numer >= 1
   {
     var f := (x: (bool, int)) => if x.0 then -x.1 else x.1;
     Monad.Map(SampleLoop(scale), f)
   }
 
-  ghost function SampleLoop(scale: Rationals.Rational): Monad.Hurd<(bool, int)>
+  ghost opaque function SampleLoop(scale: Rationals.Rational): Monad.Hurd<(bool, int)>
     requires scale.numer >= 1
   {
     Loops.While(SampleLoopCondition, SampleLoopBody(scale))((true, 0))
   }
 
-  // TODO: add correct version later
+  // TODO: replace with correct version later
   ghost function SampleLoopBody(scale: Rationals.Rational): ((bool, int)) -> Monad.Hurd<(bool, int)>
     requires scale.numer >= 1
   {
-    // replace with functional version using SampleHelper
     (x: (bool, int)) => Monad.Return(x)
   }
 
@@ -41,25 +40,18 @@ module DiscreteLaplace.Model {
     x.0 && (x.1 == 0)
   }
 
-  ghost function SampleInnerLoopFull(): Monad.Hurd<int> {
+  ghost opaque function SampleInnerLoopFull(): Monad.Hurd<int> {
     var f := (x: (bool, int)) => x.1;
     Monad.Map(SampleInnerLoop(), f)
   }
 
-  ghost function SampleInnerLoop(x: (bool, int) := (true, 0)): (f: Monad.Hurd<(bool, int)>) {
+  ghost opaque function SampleInnerLoop(x: (bool, int) := (true, 0)): Monad.Hurd<(bool, int)> {
     Loops.While(SampleInnerLoopCondition, SampleInnerLoopBody)(x)
   }
 
-  ghost function SampleInnerLoop2(x: (bool, int)): (f: Monad.Hurd<(bool, int)>)
-    ensures f == Loops.While(SampleInnerLoopCondition, SampleInnerLoopBody)(x)
-  {
-    var f := Loops.While(SampleInnerLoopCondition, SampleInnerLoopBody)(x);
-    f
-  }
-
-  ghost function SampleInnerLoopBody(x: (bool, int)): Monad.Hurd<(bool, int)> {
+  ghost opaque function SampleInnerLoopBody(x: (bool, int)): Monad.Hurd<(bool, int)> {
     Monad.Bind(
-      BernoulliExpNeg.Model.Sample(Rationals.Int(1)), 
+      BernoulliExpNeg.Model.Sample(Rationals.Int(1)),
       (a: bool) => Monad.Return((a, if a then x.1 + 1 else x.1))
     )
   }
@@ -72,7 +64,7 @@ module DiscreteLaplace.Model {
    Lemmas
   *******/
 
-  // add later
+  // TODO: add later
   lemma {:axiom} SampleInnerLoopTerminatesAlmostSurely()
     ensures Loops.WhileTerminatesAlmostSurely(SampleInnerLoopCondition, SampleInnerLoopBody)
 
